tests/lean/run/ematch1.lean
@@ -12,7 +12,7 @@ meta def add_insts : list (expr × expr) → tactic unit
 
 meta def ematch_test (h : name) (e : expr) : tactic unit :=
 do cc  ← cc_state.mk_using_hs,
-   ems ← return $ ematch_state.mk default_ematch_config,
+   ems ← return $ ematch_state.mk {},
    hlemma ← hinst_lemma.mk_from_decl h,
    (r, cc, ems) ← ematch cc ems hlemma e,
    add_insts r
