tests/lean/run/using_smt3.lean
@@ -11,11 +11,8 @@ meta def fail_if_success {α : Type} (t : smt_tactic α) : smt_tactic unit :=
 | exception .(α × smt_state) _ _ _ := success ((), ss) ts
 end
 
-def my_pre_config : smt_pre_config :=
-{ default_smt_pre_config with zeta := tt }
-
 def my_smt_config : smt_config :=
-{ default_smt_config with pre_cfg := my_pre_config }
+{ pre_cfg := { zeta := tt } }
 
 lemma ex2 : let x := 1 in ∀ y, x = y → y = 1 :=
 by using_smt_core my_smt_config $ smt_tactic.intros >> fail_if_success (get_local `x) >> return ()
