tests/lean/structure_instance_bug2.lean
@@ -1,3 +1,5 @@
+def default_smt_pre_config : smt_pre_config := {}
+
 def my_pre_config1 : smt_pre_config :=
 { default_smt_pre_config . zeta := tt }
 
